verif/verif_splitnode.v
@@ -16,6 +16,7 @@ Require Import btrees_sep.
 Require Import btrees_spec.
 Require Import verif_newnode.
 Require Import verif_findindex.
+Require Import index.
 
 Lemma body_splitnode: semax_body Vprog Gprog f_splitnode splitnode_spec.
 Proof.
@@ -26,13 +27,80 @@ Proof.
   assert(exists k, keyrepr = key_repr k).
   { destruct e; exists k; simpl; simpl in HEVR; inv HEVR; auto. }
   destruct H1 as [k HK].
-  forward.                      (* t'8=entry->key *)
-  forward_call(n,k).            (* t'1=findrecordindex(node,t'8) *)
+  forward.                      (* t'28=entry->key *)
+  forward_call(n,k).            (* t'1=findrecordindex(node,t'28) *)
   { fold n. cancel. }
   { split; auto. unfold node_wf. fold n in H0. omega. }
   forward.                      (* tgtIdx=t'1 *)
-  forward.                      (* j=0 *)
-  forward.                      (* inserted=0 *)
-  (* forward_loop *)
-  admit.
+  assert(INRANGE: 0 <= index.idx_to_Z (findRecordIndex n k) <= Z.of_nat (numKeys n)) by apply FRI_inrange.
+  fold n in H0. rewrite H0 in INRANGE.
+  rewrite unfold_btnode_rep. unfold n. Intros ent_end.
+  forward.                      (* t'27=node->Last *)
+  { destruct Last; entailer!. }
+  forward_call(isLeaf, false, Last). (* t'2=createNewNode(isLeaf,0,t'27 *)
+  Intros vnewnode.
+  forward.                      (* newnode=t'2 *)
+  gather_SEP 1 2 3 4.
+  replace_SEP 0 (btnode_rep n).
+  { entailer!. rewrite unfold_btnode_rep with (n:=n). unfold n. Exists ent_end. cancel.
+    change_compspecs CompSpecs. cancel. } clear ent_end.
+  forward_if(PROP (vnewnode<>nullval)
+     LOCAL (temp _newNode vnewnode; temp _t'2 vnewnode; temp _t'27 (Val.of_bool Last);
+     temp _tgtIdx (Vint (Int.repr (rep_index (findRecordIndex' le k (index.ip 0)))));
+     temp _t'1 (Vint (Int.repr (rep_index (findRecordIndex' le k (index.ip 0))))); 
+     temp _t'28 keyrepr; lvar _allEntries (tarray (Tstruct _Entry noattr) 16) v_allEntries;
+     temp _node nval; temp _entry pe; temp _isLeaf (Val.of_bool isLeaf))
+     SEP (btnode_rep n; btnode_rep (empty_node isLeaf false Last vnewnode);
+     data_at_ Tsh (tarray (Tstruct _Entry noattr) 16) v_allEntries; entry_rep e;
+     data_at Tsh tentry (keyrepr, coprepr) pe)).
+  { apply denote_tc_test_eq_split. replace vnewnode with (getval (empty_node isLeaf false Last vnewnode)).
+    entailer!. simpl. auto. entailer!. }
+  { forward.                    (* skip *)
+    entailer!. }
+  { assert_PROP(False). entailer!. contradiction. }
+  rewrite unfold_btnode_rep with (n:=n). unfold n. Intros ent_end.
+  forward.                      (* node->Last = 0 *)
+  forward.                      (* t'3=node->isLeaf *)
+
+  forward_if.
+
+  -                             (* Leaf Node *)
+    assert(LEAF: isLeaf=true).
+    { destruct isLeaf; auto. simpl in H2. inv H2. }
+    destruct (findRecordIndex n k) as [|fri] eqn:HFRI.
+    { simpl in INRANGE. omega. }
+    replace (findRecordIndex' le k (index.ip 0)) with (index.ip fri). simpl.
+    gather_SEP 0 1 2 3.
+    pose (nright := btnode val ptr0 le true First false nval).
+    replace_SEP 0 (btnode_rep nright).
+    { entailer!. rewrite unfold_btnode_rep with (n:=nright). unfold nright.
+      Exists ent_end. cancel. } clear ent_end. fold tentry.
+    
+    forward_for_simple_bound (Z.of_nat fri)
+    (EX i:Z, EX allent_end:list (val*(val+val)),
+     (PROP (length allent_end = (Fanout + 1 - Z.to_nat(i))%nat)
+      LOCAL (temp _t'3 (Val.of_bool isLeaf); temp _newNode vnewnode; temp _t'2 vnewnode;
+      temp _t'27 (Val.of_bool Last); temp _tgtIdx (Vint (Int.repr (Z.of_nat fri)));
+      temp _t'1 (Vint (Int.repr (Z.of_nat fri))); temp _t'28 keyrepr;
+      lvar _allEntries (tarray tentry 16) v_allEntries; temp _node nval; temp _entry pe;
+      temp _isLeaf (Val.of_bool isLeaf))
+      SEP (btnode_rep nright; btnode_rep (empty_node isLeaf false Last vnewnode);
+           data_at Tsh (tarray tentry 16) (le_to_list (nth_first_le le (Z.to_nat i))++ allent_end) v_allEntries; entry_rep e; data_at Tsh tentry (keyrepr, coprepr) pe)))%assert.
+    { simpl in INRANGE. rewrite Fanout_eq in INRANGE.
+      replace (Z.of_nat 15) with 15 in INRANGE. rep_omega. simpl. auto. }
+    { entailer!.
+      Exists (default_val (nested_field_type (tarray (Tstruct _Entry noattr) 16) [])).
+      entailer!. unfold data_at_, field_at_. entailer!. }
+    { admit.                    (* loop body *) }
+    Intros allent_end.
+    forward.                    (* t'24=entry->key *)
+    forward.                    (* allEntries[tgtIdx]->key = t'24 *)
+    { admit. }
+    forward.                    (* t'23=entry->ptr.record *)
+    { admit. }
+    forward.                    (* alentries[tgtIdx]->ptr.record=t'23 *)
+    { admit. }
+    admit.    
+  -                             (* Intern Node *)
+    admit.
 Admitted.
